Rewrite.v
@@ -2,9 +2,67 @@ Require Import List.
 Require Import Arith.
 Require Import Misc.
 Require Import Psatz.
-Require Import Star.
+
+Definition curry {A B C : Type} (f : A * B -> C) x y := f (x, y).
+Definition uncurry {A B C : Type} (f : A -> B -> C) '(x, y) := f x y.
+Definition flip {A B C : Type} (f : A -> B -> C) x y := f y x.
+Definition union {A B : Type} (R1 R2 : A -> B -> Prop) x y := R1 x y \/ R2 x y.
+Definition compose {A B C : Type} (R1 : A -> B -> Prop) (R2 : B -> C -> Prop) x y := exists z, R1 x z /\ R2 z y.
+
+Definition same_rel {A B : Type} (R1 R2 : A -> B -> Prop) :=
+  forall x y, R1 x y <-> R2 x y.
+
+Lemma same_rel_refl {A : Type} (R : A -> A -> Prop) : same_rel R R.
+Proof.
+  intros x y. reflexivity.
+Qed.
+
+Lemma same_rel_sym {A B : Type} (R1 R2 : A -> B -> Prop) :
+  same_rel R1 R2 -> same_rel R2 R1.
+Proof.
+  intros H x y; split; intros H1; apply H; assumption.
+Qed.
+
+Lemma same_rel_trans {A B : Type} (R1 R2 R3 : A -> B -> Prop) :
+  same_rel R1 R2 -> same_rel R2 R3 -> same_rel R1 R3.
+Proof.
+  intros H1 H2 x y; split; intros H3; [apply H2, H1, H3|apply H1, H2, H3].
+Qed.
+
+Lemma flip_flip :
+  forall (A B : Type) (R : A -> B -> Prop), same_rel (flip (flip R)) R.
+Proof.
+  intros A R x y. reflexivity.
+Qed.
+
+
+(* Reflexive closure *)
 
 Definition reflc {A : Type} (R : A -> A -> Prop) x y := R x y \/ x = y.
+
+Lemma same_rel_reflc {A : Type} (R1 R2 : A -> A -> Prop) :
+  same_rel R1 R2 -> same_rel (reflc R1) (reflc R2).
+Proof.
+  intros H x y.
+  split; intros [Hxy | ->]; try (right; reflexivity); left; apply H; assumption.
+Qed.
+
+
+(* Symmetric closure *)
+Definition symc {A : Type} (R : A -> A -> Prop) := union R (flip R).
+
+Lemma symc_sym {A : Type} (R : A -> A -> Prop) :
+  forall x y, symc R x y -> symc R y x.
+Proof.
+  intros x y [H | H]; [right | left]; assumption.
+Qed.
+
+
+(* Transitive reflexive closure *)
+
+Inductive star {A : Type} (R : A -> A -> Prop) : A -> A -> Prop :=
+| star_refl : forall x, star R x x
+| star_step : forall x y z, R x y -> star R y z -> star R x z.
 
 Lemma star_1 {A : Type} (R : A -> A -> Prop) :
   forall x y, R x y -> star R x y.
@@ -13,15 +71,213 @@ Proof.
   constructor.
 Qed.
 
+Lemma star_compose :
+  forall (A : Type) (R : A -> A -> Prop) x y z, star R x y -> star R y z -> star R x z.
+Proof.
+  intros A R x y z H. induction H.
+  - intros; assumption.
+  - intros; econstructor; [eassumption | firstorder].
+Qed.
+
+Lemma star_map_impl :
+  forall (A B : Type) (RA : A -> A -> Prop) (RB : B -> B -> Prop) (f : A -> B),
+    (forall x y, RA x y -> RB (f x) (f y)) -> forall x y, star RA x y -> star RB (f x) (f y).
+Proof.
+  intros A B RA RB f HR x y H. induction H.
+  - constructor.
+  - econstructor; eauto.
+Qed.
+
+Lemma star_impl :
+  forall (A : Type) (R1 R2 : A -> A -> Prop),
+    (forall x y, R1 x y -> R2 x y) -> forall x y, star R1 x y -> star R2 x y.
+Proof.
+  intros A R1 R2 H x y Hxy. eapply star_map_impl with (f := id); eassumption.
+Qed.
+
+Lemma same_rel_star {A : Type} (R1 R2 : A -> A -> Prop) :
+  same_rel R1 R2 -> same_rel (star R1) (star R2).
+Proof.
+  intros H x y.
+  split; intros Hxy; eapply star_impl; try eassumption; intros; apply H; assumption.
+Qed.
+
+Lemma flip_star :
+  forall (A : Type) (R : A -> A -> Prop) x y, star (flip R) x y -> star R y x.
+Proof.
+  intros A R x y H. induction H.
+  - apply star_refl.
+  - eapply star_compose; [eassumption|]. apply star_1; assumption.
+Qed.
+
+Lemma flip_star_iff :
+  forall (A : Type) (R : A -> A -> Prop), same_rel (star (flip R)) (flip (star R)).
+Proof.
+  intros A R x y; split; intros H.
+  - apply flip_star. assumption.
+  - eapply flip_star, same_rel_star; [|eassumption]. apply flip_flip.
+Qed.
+
+Lemma star_star :
+  forall (A : Type) (R : A -> A -> Prop), forall x y, star (star R) x y -> star R x y.
+Proof.
+  intros A R x y H. induction H.
+  - constructor.
+  - eapply star_compose; eauto.
+Qed.
+
+Lemma star_induction_rev :
+  forall {A : Type} (R : A -> A -> Prop) (P : A -> Prop) (x : A),
+    P x -> (forall y z, P y -> R y z -> P z) -> (forall y, star R x y -> P y).
+Proof.
+  intros A R P x HPx HPind y Hy. revert HPx.
+  induction Hy; firstorder.
+Qed.
+
+Lemma star_same :
+  forall (A : Type) (R : A -> A -> Prop) t1 t2, t1 = t2 -> star R t1 t2.
+Proof.
+  intros A R t1 t2 ->. constructor.
+Qed.
+
+Lemma star_sym {A : Type} (R : A -> A -> Prop) (Hsym : forall x y, R x y -> R y x) :
+  forall x y, star R x y -> star R y x.
+Proof.
+  intros x y H; induction H.
+  - apply star_refl.
+  - eapply star_compose; [eassumption|apply star_1, Hsym; assumption].
+Qed.
+
 Lemma reflc_star {A : Type} (R : A -> A -> Prop) :
   forall x y, reflc R x y -> star R x y.
 Proof.
   intros x y [Hxy | <-]; [apply star_1; assumption|constructor].
 Qed.
 
-Definition union {A : Type} (R1 R2 : A -> A -> Prop) (x y : A) := R1 x y \/ R2 x y.
+Lemma star_reflc {A : Type} (R : A -> A -> Prop) :
+  same_rel (star R) (star (reflc R)).
+Proof.
+  intros x y. split; intros H.
+  - eapply star_impl; [|eassumption].
+    intros; left; assumption.
+  - induction H.
+    + constructor.
+    + destruct H as [H | ->].
+      * econstructor; eassumption.
+      * assumption.
+Qed.
 
-Definition compose {A : Type} (R1 R2 : A -> A -> Prop) (x y : A) := exists z, R1 x z /\ R2 z y.
+(* Transitive closure *)
+
+Inductive plus {A : Type} (R : A -> A -> Prop) : A -> A -> Prop :=
+| plus_1 : forall x y, R x y -> plus R x y
+| plus_S : forall x y z, R x y -> plus R y z -> plus R x z.
+
+Lemma plus_map_impl :
+  forall (A B : Type) (RA : A -> A -> Prop) (RB : B -> B -> Prop) (f : A -> B),
+    (forall x y, RA x y -> RB (f x) (f y)) -> forall x y, plus RA x y -> plus RB (f x) (f y).
+Proof.
+  intros A B RA RB f HR x y H. induction H.
+  - apply plus_1; auto.
+  - eapply plus_S; eauto.
+Qed.
+
+Lemma plus_impl :
+  forall (A : Type) (R1 R2 : A -> A -> Prop),
+    (forall x y, R1 x y -> R2 x y) -> forall x y, plus R1 x y -> plus R2 x y.
+Proof.
+  intros A R1 R2 H x y Hxy. eapply plus_map_impl with (f := id); eassumption.
+Qed.
+
+Lemma same_rel_plus :
+  forall (A : Type) (R1 R2 : A -> A -> Prop), same_rel R1 R2 -> same_rel (plus R1) (plus R2).
+Proof.
+  intros A R1 R2 H x y. split; intros Hplus; eapply plus_impl; try eassumption; intros; apply H; assumption.
+Qed.
+
+Lemma plus_star :
+  forall (A : Type) (R : A -> A -> Prop) x y, plus R x y -> star R x y.
+Proof.
+  intros A R x y H; induction H.
+  - apply star_1. assumption.
+  - econstructor; eassumption.
+Qed.
+
+Lemma plus_star_iff :
+  forall (A : Type) (R : A -> A -> Prop), same_rel (plus R) (compose R (star R)).
+Proof.
+  intros A R x y; split; intros H.
+  - inversion H; subst.
+    + exists y; split; [assumption|apply star_refl].
+    + exists y0. split; [assumption|apply plus_star; assumption].
+  - destruct H as (z & Hxz & Hzy).
+    revert x Hxz; induction Hzy; intros w Hw.
+    + apply plus_1; assumption.
+    + eapply plus_S; [eassumption|apply IHHzy; assumption].
+Qed.
+
+Lemma plus_compose_star_left :
+  forall (A : Type) (R : A -> A -> Prop) x y z, star R x y -> plus R y z -> plus R x z.
+Proof.
+  intros A R x y z H1 H2; induction H1; [assumption|].
+  econstructor; [eassumption|].
+  apply IHstar; assumption.
+Qed.
+
+Lemma flip_plus :
+  forall (A : Type) (R : A -> A -> Prop) x y, plus (flip R) x y -> plus R y x.
+Proof.
+  intros A R x y H. induction H.
+  - apply plus_1. assumption.
+  - eapply plus_compose_star_left; [eapply plus_star; eassumption|].
+    apply plus_1. assumption.
+Qed.
+
+Lemma flip_plus_iff :
+  forall (A : Type) (R : A -> A -> Prop), same_rel (plus (flip R)) (flip (plus R)).
+Proof.
+  intros A R x y; split; intros H.
+  - apply flip_plus. assumption.
+  - eapply flip_plus, same_rel_plus; [|eassumption]. apply flip_flip.
+Qed.
+
+Lemma plus_compose_star_right :
+  forall (A : Type) (R : A -> A -> Prop) x y z, plus R x y -> star R y z -> plus R x z.
+Proof.
+  intros A R x y z H1 H2.
+  apply flip_plus_iff.
+  eapply plus_compose_star_left; [|apply flip_plus_iff; eassumption].
+  apply flip_star in H2. eassumption.
+Qed.
+
+
+(* Transitive symmetric reflexive closure *)
+
+Definition convertible {A : Type} (R : A -> A -> Prop) := star (symc R).
+
+Lemma convertible_refl {A : Type} (R : A -> A -> Prop) x : convertible R x x.
+Proof.
+  intros; apply star_refl.
+Qed.
+
+Lemma convertible_sym {A : Type} (R : A -> A -> Prop) :
+  forall x y, convertible R x y -> convertible R y x.
+Proof.
+  apply star_sym, symc_sym.
+Qed.
+
+Lemma common_reduce_convertible :
+  forall (A : Type) (R : A -> A -> Prop) x y z, star R x z -> star R y z -> convertible R x y.
+Proof.
+  intros A R x y z Hxz Hyz.
+  eapply star_compose.
+  - eapply star_impl; [|eassumption]. intros; left; assumption.
+  - eapply star_impl; [|apply flip_star_iff; eassumption]. intros; right; assumption.
+Qed.
+
+
+
+(* Confluence *)
 
 Definition commuting_diamond {A : Type} (R1 R2 : A -> A -> Prop) :=
   forall x y z, R1 x y -> R2 x z -> exists w, R2 y w /\ R1 z w.
@@ -46,28 +302,6 @@ Lemma commute_symmetric {A : Type} (R1 R2 : A -> A -> Prop) :
   commute R1 R2 -> commute R2 R1.
 Proof.
   intros. apply commuting_diamond_symmetric. assumption.
-Qed.
-
-Definition same_rel {A : Type} (R1 R2 : A -> A -> Prop) :=
-  forall x y, R1 x y <-> R2 x y.
-
-Lemma same_rel_refl {A : Type} (R : A -> A -> Prop) : same_rel R R.
-Proof.
-  intros x y. reflexivity.
-Qed.
-
-Lemma same_rel_star {A : Type} (R1 R2 : A -> A -> Prop) :
-  same_rel R1 R2 -> same_rel (star R1) (star R2).
-Proof.
-  intros H x y.
-  split; intros Hxy; eapply star_map_impl with (f := id); try eassumption; intros; apply H; assumption.
-Qed.
-
-Lemma same_rel_reflc {A : Type} (R1 R2 : A -> A -> Prop) :
-  same_rel R1 R2 -> same_rel (reflc R1) (reflc R2).
-Proof.
-  intros H x y.
-  split; intros [Hxy | ->]; try (right; reflexivity); left; apply H; assumption.
 Qed.
 
 Lemma commuting_diamond_ext {A : Type} (R1a R2a R1b R2b : A -> A -> Prop) :
@@ -147,9 +381,34 @@ Lemma between_star {A : Type} (R1 R2 : A -> A -> Prop) :
   (forall x y, R1 x y -> R2 x y) -> (forall x y, R2 x y -> star R1 x y) -> same_rel (star R1) (star R2).
 Proof.
   intros H1 H2 x y. split; intros H.
-  - eapply star_map_impl with (f := id); eassumption.
+  - eapply star_impl; eassumption.
   - eapply star_star.
-    eapply star_map_impl with (f := id); eassumption.
+    eapply star_impl; eassumption.
+Qed.
+
+Definition weak_diamond {A : Type} (R : A -> A -> Prop) :=
+  forall x y z, R x y -> R x z -> y = z \/ (exists w, R y w /\ R z w).
+
+Lemma weak_diamond_diamond_reflc {A : Type} (R : A -> A -> Prop) :
+  weak_diamond R -> diamond (reflc R).
+Proof.
+  intros HD x y z [Hxy | <-] [Hxz | <-].
+  - specialize (HD x y z Hxy Hxz).
+    destruct HD as [-> | (w & Hyw & Hzw)].
+    + exists z. split; right; reflexivity.
+    + exists w. split; left; assumption.
+  - exists y. split; [right; reflexivity|left; assumption].
+  - exists z. split; [left; assumption|right; reflexivity].
+  - exists x. split; right; reflexivity.
+Qed.
+
+Lemma weak_diamond_confluent {A : Type} (R : A -> A -> Prop) :
+  weak_diamond R -> confluent R.
+Proof.
+  intros H.
+  apply weak_diamond_diamond_reflc, diamond_is_confluent in H.
+  eapply diamond_ext; [|eassumption].
+  apply star_reflc.
 Qed.
 
 
@@ -169,7 +428,23 @@ Proof.
     eapply diamond_ext; [|exact H]. apply between_star.
     + intros x y [H1 | H2]; [exists y|exists x]; split; econstructor; try eassumption; constructor.
     + intros x z (y & Hxy & Hyz).
-      eapply star_compose; eapply star_map_impl with (f := id); try eassumption;
+      eapply star_compose; eapply star_impl; try eassumption;
         intros u v Huv; [left|right]; assumption.
 Qed.
 
+
+Lemma convertible_confluent_common_reduce :
+  forall (A : Type) (R : A -> A -> Prop),
+    confluent R -> forall x y, convertible R x y -> exists z, star R x z /\ star R y z.
+Proof.
+  intros A R Hconf x y Hconv. induction Hconv.
+  - exists x. split; constructor.
+  - destruct IHHconv as (w & Hyw & Hzw).
+    destruct H as [Hxy | Hyx].
+    + exists w. split; [|assumption]. econstructor; eassumption.
+    + destruct (Hconf y x w) as (t & Hxt & Hwt).
+      * apply star_1. assumption.
+      * assumption.
+      * exists t. split; [assumption|].
+        eapply star_compose; eassumption.
+Qed.
