GenInd.v
@@ -1,0 +1,433 @@
+From Ltac2 Require Import Ltac2.
+
+Require Import List.
+Require Import Misc.
+Require Import STerm. (* for testing *)
+
+Set Ltac2 Backtrace.
+
+Ltac2 eassumption_tac () := ltac1:(eassumption).
+Ltac2 Notation eassumption := eassumption_tac ().
+
+Definition proj1_transparent {A B : Prop} (H : A /\ B) : A := match H with conj P Q => P end.
+Definition proj2_transparent {A B : Prop} (H : A /\ B) : B := match H with conj P Q => Q end.
+
+Lemma Exists_impl_transparent :
+  forall (A : Type) (P Q : A -> Prop) (L : list A), (forall x, P x -> Q x) -> Exists P L -> Exists Q L.
+Proof.
+  intros A P Q L H1 H2. induction H2.
+  - apply Exists_cons_hd, H1. assumption.
+  - apply Exists_cons_tl, IHExists.
+Defined.
+
+Lemma Exists_impl_strong_transparent :
+  forall (A : Type) (P Q : A -> Prop) (L : list A), (forall x, P x -> Q x) -> Exists P L -> Exists (fun x => P x /\ Q x) L.
+Proof.
+  intros A P Q L H1 H2. eapply Exists_impl_transparent > [|eassumption].
+  intros x Hx; split > [apply Hx|apply H1, Hx].
+Defined.
+
+Ltac2 get_binder_maybe (c : constr) :=
+  match Constr.Unsafe.kind c with
+  | Constr.Unsafe.Prod b _ => Some b
+  | Constr.Unsafe.Lambda b _ => Some b
+  | Constr.Unsafe.LetIn b _ _ => Some b
+  | _ => None
+  end.
+
+Ltac2 get_binder (c : constr) :=
+  match get_binder_maybe c with
+  | Some b => b
+  | None => Control.throw (Invalid_argument (Some (Message.of_constr c)))
+  end.
+
+Ltac2 head_binder_ident (c : constr) :=
+  Fresh.in_goal (
+      match get_binder_maybe c with
+      | None => @_x
+      | Some b =>
+        match Constr.Binder.name b with
+        | None => @_x
+        | Some x => x
+        end
+      end).
+
+Ltac2 rec rebuild_lam (t : constr) :=
+  match Constr.Unsafe.kind t with
+  | Constr.Unsafe.Lambda b t1 => Constr.Unsafe.make (Constr.Unsafe.Lambda b (rebuild_lam t1))
+  | _ => t
+  end.
+
+Ltac2 inctx (name : ident) (t : constr) (body : constr -> constr) :=
+  Constr.in_context name t (fun () => Control.refine (fun () => body (Control.hyp name))).
+
+Ltac2 make_forall (c : constr) :=
+  match Constr.Unsafe.kind c with
+  | Constr.Unsafe.Lambda b t => Constr.Unsafe.make (Constr.Unsafe.Prod b t)
+  | _ => Control.throw (Invalid_argument (Some (Message.of_constr c)))
+  end.
+
+Ltac2 mk_app (u : constr) (v : constr) := '($u $v).
+Ltac2 mk_app2 (u : constr) (v : constr) (w : constr) := '($u $v $w).
+Ltac2 mk_app3 (u : constr) (v : constr) (w : constr) (x : constr) := '($u $v $w $x).
+
+Ltac2 mk_forall_proof_smart (x : ident) (u : constr) (v : constr -> constr) :=
+  lazy_match! (Std.eval_hnf u) with
+  | True => v 'I
+  | ?u =>
+    let vx := inctx x u v in
+    lazy_match! (Std.eval_hnf (Constr.type vx)) with
+    | (_ -> True) => 'I
+    | _ => vx
+    end
+  end.
+
+Ltac2 mk_Forall_proof_smart (x : ident) (t : constr) (u : constr -> constr) (v : constr) :=
+  let ux := inctx x t u in
+  lazy_match! (Std.eval_hnf (Constr.type ux)) with
+  | (_ -> True) => 'I
+  | _ => '(Forall_True_transparent $t _ $v $ux)
+  end.
+
+Ltac2 mk_and_proof_smart (u : constr) (v : constr) :=
+  let ut := Std.eval_hnf (Constr.type u) in
+  let vt := Std.eval_hnf (Constr.type v) in
+  lazy_match! '($ut /\ $vt) with
+  | True /\ _ => v
+  | _ /\ True => u
+  | _ => '(conj _ _ $u $v)
+  end.
+
+
+Ltac2 mk_Forall_impl_smart (t : constr) (p : constr) (l : constr) (u : constr -> constr) (v : constr) :=
+  let ux := inctx (head_binder_ident p) t (fun xx => inctx (Fresh.in_goal @H) (mk_app p xx) u) in
+  lazy_match! (Std.eval_hnf (Constr.type ux)) with
+  | (forall x H, True) => 'I
+  | _ => '(Forall_impl_transparent $t _ _ $l $ux $v)
+  end.
+
+Ltac2 mk_Forall2_impl_smart (t1 : constr) (t2 : constr) (p : constr) (l1 : constr) (l2 : constr) (u : constr -> constr) (v : constr) :=
+  let ux := inctx (head_binder_ident p) t1 (fun xx =>
+    let y := head_binder_ident (Std.eval_hnf (mk_app p xx)) in
+    inctx y t2 (fun yy =>
+      inctx (Fresh.in_goal @H) (mk_app (mk_app p xx) yy) u)) in
+  lazy_match! (Std.eval_hnf (Constr.type ux)) with
+  | (forall x y H, True) => 'I
+  | _ => '(Forall2_impl_transparent $t1 $t2 _ _ $l1 $l2 $ux $v)
+  end.
+
+Ltac2 mk_Exists_impl_smart (t : constr) (p : constr) (l : constr) (u : constr -> constr) (v : constr) :=
+  let ux := inctx (head_binder_ident p) t (fun xx => inctx (Fresh.in_goal @H) (mk_app p xx) u) in
+  lazy_match! (Std.eval_hnf (Constr.type ux)) with
+  | (forall x H, True) => 'I
+  | _ => '(Exists_impl_strong_transparent $t _ _ $l $ux $v)
+  end.
+
+
+Ltac2 message_concat_list (l : message list) :=
+  List.fold_left (fun m1 m2 => Message.concat m1 m2) l (Message.of_string "").
+
+Ltac2 message_of_hyps () :=
+  message_concat_list (List.map (fun (id, _, c) => message_concat_list [Message.of_ident id; Message.of_string " : "; Message.of_constr c; Message.of_string "
+"]) (Control.hyps ())).
+
+Ltac2 typed_constr_message (c : constr) :=
+  Message.concat (Message.concat (Message.of_constr c) (Message.of_string " : ")) (Message.of_constr (Constr.type c)).
+Ltac2 log (c : constr) := Message.print (typed_constr_message c).
+Ltac2 logged (r : constr) := log r; r.
+Ltac2 log_context () := Message.print (Message.of_string "Context:"); Message.print (message_of_hyps ()).
+
+Ltac2 rec is_ind_prefix (ind : constr) (t : constr) (args : constr list) :=
+  (* Assumes t is in hnf *)
+  if Constr.equal t ind then
+    Some (List.rev args)
+  else
+    lazy_match! t with
+    | ?t1 ?t2 => is_ind_prefix ind t1 (t2 :: args)
+    | _ => None
+    end.
+
+Ltac2 rec is_ind_prefix_l (inds : constr list) (t : constr) (l : 'a list) :=
+  match inds with
+  | [] => None
+  | ind :: inds =>
+    match is_ind_prefix ind t [] with
+    | Some args => Some (args, List.hd l)
+    | None => is_ind_prefix_l inds t (List.tl l)
+    end
+  end.
+
+Ltac2 rec applist (c : constr) (l : constr list) :=
+  match l with
+  | [] => c
+  | x :: l => mk_app (applist c l) x
+  end.
+
+Ltac2 rec constrind_hyp (v : constr) (inds : constr list) (hrecs : constr list) :=
+  let t := Std.eval_hnf (Constr.type v) in
+  match is_ind_prefix_l inds t hrecs with
+  | Some argshrec => let (args, hrec) := argshrec in mk_app (applist hrec args) v
+  | None =>
+    lazy_match! t with
+    | list ?a => mk_Forall_proof_smart (Fresh.in_goal @x) a (fun x => constrind_hyp x inds hrecs) v
+    | @Forall ?t ?p ?l =>
+      mk_Forall_impl_smart t p l (fun h => constrind_hyp h inds hrecs) v
+    | @Forall2 ?t1 ?t2 ?p ?l1 ?l2 =>
+      mk_Forall2_impl_smart t1 t2 p l1 l2 (fun h => constrind_hyp h inds hrecs) v
+    | @Exists ?t ?p ?l =>
+      mk_Exists_impl_smart t p l (fun h => constrind_hyp h inds hrecs) v
+    | (?a * ?b)%type =>
+      mk_and_proof_smart
+        (constrind_hyp (mk_app 'fst v) inds hrecs)
+        (constrind_hyp (mk_app 'snd v) inds hrecs)
+    | ?a /\ ?b =>
+      mk_and_proof_smart
+        (constrind_hyp (mk_app 'proj1_transparent v) inds hrecs)
+        (constrind_hyp (mk_app 'proj2_transparent v) inds hrecs)
+    | forall (x : ?t1), @?t2 x =>
+      mk_forall_proof_smart (head_binder_ident t) t1 (fun x => constrind_hyp (mk_app v x) inds hrecs)
+    | _ => 'I
+    end
+  end.
+
+Ltac2 add1 (t : constr) (l : constr list) :=
+  lazy_match! (Std.eval_hnf (Constr.type t)) with
+  | True => l
+  | _ => t :: l
+  end.
+
+Ltac2 maybe_app (t1 : constr) (t2 : constr) :=
+  lazy_match! (Constr.type (Constr.type t2)) with
+  | Prop => t1
+  | _ => mk_app t1 t2
+  end.
+
+Ltac2 rec constrind1 (c : constr) (cstr : constr) (cstrhyp : constr) (inds : constr list) (ps : constr list) (hrecs : constr list) (args : constr list) (args_recs : constr list) :=
+  let c := Std.eval_hnf c in
+  lazy_match! c with
+  | forall (x : ?t1), @?t2 x =>
+    let x := head_binder_ident c in
+    inctx x t1 (fun xx =>
+      constrind1 (mk_app t2 xx) cstr cstrhyp inds ps hrecs (xx :: args) (add1 (constrind_hyp xx inds hrecs) args_recs)
+    )
+  | ?c =>
+    let nt := applist (applist cstrhyp args) args_recs in
+    match is_ind_prefix_l inds (Constr.type (applist cstr args)) ps with
+    | None => Control.throw Assertion_failure
+    | Some targsp =>
+      let (targs, p) := targsp in
+      Std.unify (Constr.type nt) (maybe_app (applist p targs) (applist cstr args));
+      nt
+    end
+  end.
+
+Ltac2 get_constructors_base (ind : inductive) (inst : instance) (args : constr list) :=
+  List.init (Ind.nconstructors (Ind.data ind))
+            (fun i => let c := Ind.get_constructor (Ind.data ind) i in
+                   applist (Constr.Unsafe.make (Constr.Unsafe.Constructor c inst)) args
+            ).
+
+Ltac2 rec split_ind (c : constr) (args : constr list) :=
+  lazy_match! (Std.eval_hnf c) with
+  | ?t1 ?t2 => split_ind t1 (t2 :: args)
+  | ?c => match Constr.Unsafe.kind c with
+         | Constr.Unsafe.Ind ind inst => (ind, inst, args)
+         | _ => Control.throw (Invalid_argument (Some (Message.of_constr c)))
+         end
+  end.
+
+Ltac2 get_constructors (c : constr) :=
+  let (ind, inst, args) := split_ind c [] in
+  get_constructors_base ind inst args.
+
+(*
+Ltac2 rec copy_string_from (s1 : string) (s2 : string) (i : int) (j : int) :=
+  if Int.equal i (String.length s1) then () else (
+      String.set s2 j (String.get s1 i);
+      copy_string_from s1 s2 (Int.add i 1) (Int.add j 1)
+    ).
+
+Ltac2 concat_string (s1 : string) (s2 : string) :=
+  let s3 := String.make (Int.add (String.length s1) (String.length s2)) (Char.of_int 0) in
+  copy_string_from s1 s3 0 0;
+  copy_string_from s2 s3 0 (String.length s1);
+  s3.
+
+Ltac2 named_ident (s : string) := match Ident.of_string s with Some i => i | None => @_unnamed_ end.
+ *)
+
+Ltac2 rec ncontext (l : constr list) (l2 : constr list) (tac : constr list -> constr) :=
+  match l with
+  | [] => tac (List.rev l2)
+  | _ :: l => inctx (Fresh.in_goal @H) '(_ : Prop) (fun h => ncontext l (h :: l2) tac)
+  end.
+
+Ltac2 rec nabs (n : int) (c : constr) :=
+  if Int.equal n 0 then c else '(fun _ => ltac2:(Control.refine (fun () => nabs (Int.sub n 1) c))).
+
+Ltac2 rec ind_principle_p (t : constr) :=
+  lazy_match! (Constr.type t) with
+  | forall (x : ?t1), _ =>
+    let x := head_binder_ident (Constr.type t) in
+    make_forall (inctx x t1 (fun xx => ind_principle_p (mk_app t xx)))
+  | Set => '($t -> Prop)
+  | Type => '($t -> Prop)
+  | Prop => 'Prop
+  end.
+
+Ltac2 rec forall_principle (t : constr) (p : constr) :=
+  lazy_match! (Constr.type t) with
+  | forall (x : ?t1), _ =>
+    let x := head_binder_ident (Constr.type t) in
+    make_forall (inctx x t1 (fun xx => forall_principle (mk_app t xx) (mk_app p xx)))
+  | Set => '(forall (t : $t), $p t)
+  | Type => '(forall (t : $t), $p t)
+  | Prop => '($t -> $p)
+end.
+
+Ltac2 rec intro_hyp (name : ident) (c : constr) (tac : constr -> constr) :=
+  lazy_match! (Constr.type c) with
+  | forall (x : ?t1), _ =>
+    inctx (head_binder_ident (Constr.type c)) t1 (fun xx => intro_hyp name (mk_app c xx) tac)
+  | _ => inctx name c tac
+  end.
+
+Ltac2 rec rec_pos (t : constr) :=
+  match Constr.Unsafe.kind t with
+  | Constr.Unsafe.Prod _ t => Int.add 1 (rec_pos t)
+  | _ => 0
+  end.
+
+Ltac2 rec eta_expand (c : constr) (p : constr) :=
+  lazy_match! (Constr.type c) with
+  | forall (x : ?t1), _ =>
+    let x := head_binder_ident (Constr.type c) in
+    inctx x t1 (fun xx => eta_expand (mk_app c xx) (mk_app p xx))
+  | Prop => '(fun (_ : $c) => $p)
+  | Set => '(fun (t : $c) => $p t)
+  | Type => '(fun (t : $c) => $p t)
+  end.
+
+Ltac2 rec fresh_n (n : int) (x : ident) (s : Fresh.Free.t) :=
+  if Int.equal n 0 then [] else
+    let y := Fresh.fresh s x in
+    y :: fresh_n (Int.sub n 1) x (Fresh.Free.union s (Fresh.Free.of_ids [y])).
+
+Ltac2 rec fresh_n_goal (n : int) (x : ident) := fresh_n n x (Fresh.Free.of_goal ()).
+
+Ltac2 inctxn (names : ident list) (ts : constr list) (body : constr list -> constr) :=
+  List.fold_right2 (fun name t tac l => inctx name t (fun x => tac (x :: l))) (fun l => body (List.rev l)) names ts [].
+
+Ltac2 ncontext_l (cstrsl : constr list list) (body : constr list list -> constr) :=
+  List.fold_right (fun cstrs tac lhl => ncontext cstrs [] (fun lhyps => tac (lhyps :: lhl))) (fun l => body (List.rev l)) cstrsl [].
+
+Ltac2 mkfix1 (guarded_arg : int) (name : ident) (t : constr) (body : constr -> constr) :=
+  let (b, body) :=
+      match Constr.Unsafe.kind (inctx name t body) with
+      | Constr.Unsafe.Lambda b body => (b, body)
+      | _ => Control.throw Assertion_failure
+      end
+  in
+  Constr.Unsafe.make (Constr.Unsafe.Fix (Array.make 1 guarded_arg) 0 (Array.make 1 b) (Array.make 1 body)).
+
+Ltac2 rec get_body (names : ident list) (bds : binder list) (t : constr) :=
+  match names with
+  | [] => (List.rev bds, t)
+  | _ :: names =>
+    match Constr.Unsafe.kind t with
+    | Constr.Unsafe.Lambda b body => get_body names (b :: bds) body
+    | _ => Control.throw Assertion_failure
+    end
+  end.
+
+Ltac2 mkprod u v := '($u, $v).
+
+Ltac2 rec mkprodn (l : constr list) :=
+  match List.tl l with
+  | [] => List.hd l
+  | _ => mkprod (List.hd l) (mkprodn (List.tl l))
+  end.
+
+Ltac2 mkfix (guarded_arg : int list) (names : ident list) (ts : constr list) (body : (constr list -> constr) list) :=
+  let bodies := List.map (inctxn names ts) body in
+  let (binders, _) := get_body names [] (List.hd bodies) in
+  let binders := Array.of_list binders in
+  let guarded_arg := Array.of_list guarded_arg in
+  let bodies := Array.of_list (List.map (fun body => let (_, body) := (get_body names [] body) in body) bodies) in
+  mkprodn (List.init (List.length names) (fun n => Constr.Unsafe.make (Constr.Unsafe.Fix guarded_arg n binders bodies))).
+
+Ltac2 map3 f l1 l2 l3 := List.map2 (fun a (b, c) => f a b c) l1 (List.combine l2 l3).
+Ltac2 map4 f l1 l2 l3 l4 := map3 (fun a b (c, d) => f a b c d) l1 l2 (List.combine l3 l4).
+Ltac2 map5 f l1 l2 l3 l4 l5 := map4 (fun a b c (d, e) => f a b c d e) l1 l2 l3 (List.combine l4 l5).
+
+Ltac2 gen_ind_principle (cl : constr list) :=
+  let n := List.length cl in
+  let indstl := List.map (fun c => split_ind c []) cl in
+  let cstrsl := List.map (fun (ind, inst, args) => get_constructors_base ind inst args) indstl in
+  inctxn (fresh_n_goal n @P) (List.map ind_principle_p cl) (fun pl =>
+    ncontext_l cstrsl (fun lhypsl =>
+      mkfix (List.map (fun c => rec_pos (Constr.type c)) cl) (fresh_n_goal n @Hrec) (List.map2 forall_principle cl pl)
+            (map5 (fun c (ind, _, _) => fun p cstrs lhyps hrecs =>
+        intro_hyp (Fresh.in_goal @x) c (fun xx =>
+          let branches := List.map2 (fun cstr hcstr => rebuild_lam (constrind1 (Constr.type cstr) cstr hcstr cl pl hrecs [] [])) cstrs lhyps in
+          Constr.Unsafe.make
+            (Constr.Unsafe.Case
+               (Constr.Unsafe.case ind)
+               (rebuild_lam (eta_expand c p))
+               Constr.Unsafe.NoInvert
+               xx
+               (Array.of_list branches))
+         )) cl indstl pl cstrsl lhypsl)
+    )
+  ).
+
+
+Inductive A : Type -> Prop :=
+| mkt : nat -> A nat -> A bool.
+
+Inductive L (A : Type) : Type :=
+  C : A -> list A -> L A -> list (L A) -> L A * nat -> list (L A * nat) -> (forall n m, n + m = m + n -> L A) -> L A.
+
+Inductive even : nat -> Prop :=
+| even_O : even O
+| even_S : forall n, odd n -> even (S n)
+
+with odd : nat -> Prop :=
+| odd_S : forall n, even n -> odd (S n).
+
+Notation "'Induction' 'For' [ x ]" := ltac2:(let l := [x] in Control.refine (fun () => gen_ind_principle (List.map Constr.pretype l))) (at level 0, only parsing).
+Notation "'Induction' 'For' [ x ; y ]" :=
+  ltac2:(let l := [x; y] in Control.refine (fun () => gen_ind_principle (List.map Constr.pretype l))) (at level 0, only parsing).
+Notation "'Induction' 'For' [ x ; y ; z ]" :=
+  ltac2:(let l := [x; y; z] in Control.refine (fun () => gen_ind_principle (List.map Constr.pretype l))) (at level 0, only parsing).
+Notation "'Induction' 'For' [ x ; y ; z ; w ]" :=
+  ltac2:(let l := [x; y; z; w] in Control.refine (fun () => gen_ind_principle (List.map Constr.pretype l))) (at level 0, only parsing).
+Notation "'Induction' 'For' [ x ; y ; z ; w ; t ]" :=
+  ltac2:(let l := [x; y; z; w; t] in Control.refine (fun () => gen_ind_principle (List.map Constr.pretype l))) (at level 0, only parsing).
+
+Definition L_ind2 (A : Type) := Induction For [ L A ].
+Definition term_ind3 := Induction For [ term ].
+Definition test := Induction For [ A ].
+Definition testeven := Induction For [ even ; odd ].
+
+Inductive t : term -> Prop :=
+| t_var : forall n, t (var n)
+| t_constr : forall tag l, Exists t l -> t (constr tag l).
+Definition test3 := Induction For [ t ].
+Print test3.
+
+Inductive pbeta : term -> term -> Prop :=
+| pbeta_var : forall n, pbeta (var n) (var n)
+| pbeta_dvar : forall n, pbeta (dvar n) (dvar n)
+| pbeta_app : forall t1 t2 t3 t4, pbeta t1 t2 -> pbeta t3 t4 -> pbeta (app t1 t3) (app t2 t4)
+| pbeta_redex : forall t1 t2 t3 t4, pbeta t1 t2 -> pbeta t3 t4 -> pbeta (app (abs t1) t3) (subst1 t4 t2)
+| pbeta_abs : forall t1 t2, pbeta t1 t2 -> pbeta (abs t1) (abs t2)
+| pbeta_constr : forall tag l1 l2, Forall2 pbeta l1 l2 -> pbeta (constr tag l1) (constr tag l2)
+| pbeta_switch : forall t1 t2 l1 l2, pbeta t1 t2 -> Forall2 (fun pt1 pt2 => fst pt1 = fst pt2 /\ pbeta (snd pt1) (snd pt2)) l1 l2 -> pbeta (switch t1 l1) (switch t2 l2)
+| pbeta_switch_redex : forall lt1 lt2 t1 t2 l1 l2,
+    Forall2 pbeta lt1 lt2 -> pbeta t1 t2 ->
+    pbeta (switch (constr (length l1) lt1) (l1 ++ (length lt1, t1) :: l2)) (subst (read_env lt2) t2).
+
+Definition test2 := Induction For [ pbeta ].
+Check test2.
+
